added first version of ideal_eval for ultimate_slh and 'ultimate_slh_bcc' lemma with a few proven cases

UltimateSLH.v
@@ -51,8 +51,6 @@ Definition relative_secure (trans : com -> com) (c:com) (st1 st2:state) : Prop :
 Definition BOr b1 b2 := BNot (BAnd (BNot b1) (BNot b2)).
 Notation "x || y"  := (BOr x y) (in custom com at level 80, left associativity). *)
 
-Axiom MASK : nat.
-
 Fixpoint ultimate_slh (c:com) :=
   (match c with
   | <{{skip}}> => <{{skip}}>
@@ -100,11 +98,69 @@ Proof.
   apply observations_fixed in H2; try auto. congruence.
 Qed.
 
-(* TODO: this should be defined wrt a new ideal semantics for Ultimate SLH *)
-Definition ideal_spec_obs_secure c st1 st2 ast1 ast2 : Prop :=
+Reserved Notation
+         "'|-ideal-' '<(' st , ast , b , ds ')>' '=[' c ']=>' '<(' stt , astt , bb , os ')>'"
+         (at level 40, c custom com at level 99,
+          st constr, ast constr, stt constr, astt constr at next level).
+
+Inductive ideal_eval :
+    com -> state -> astate -> bool -> dirs ->
+           state -> astate -> bool -> obs -> Prop :=
+  | Ideal_Skip : forall st ast b,
+      |-ideal- <(st, ast, b, [])> =[ skip ]=> <(st, ast, b, [])>
+  | Ideal_Asgn  : forall st ast b e n x,
+      aeval st e = n ->
+      |-ideal- <(st, ast, b, [])> =[ x := e ]=> <(x !-> n; st, ast, b, [])>
+  | Ideal_Seq : forall c1 c2 st ast b st' ast' b' st'' ast'' b'' os1 os2 ds1 ds2,
+      |-ideal- <(st, ast, b, ds1)> =[ c1 ]=> <(st', ast', b', os1)>  ->
+      |-ideal- <(st', ast', b', ds2)> =[ c2 ]=> <(st'', ast'', b'', os2)> ->
+      |-ideal- <(st, ast, b, ds1++ds2)>  =[ c1 ; c2 ]=> <(st'', ast'', b'', os2++os1)>
+  | Ideal_If : forall st ast b st' ast' b' be c1 c2 os1 ds,
+      |-ideal- <(st, ast, b, ds)> =[ match beval st be && (negb b) with
+                                 | true => c1
+                                 | false => c2 end ]=> <(st', ast', b', os1)> ->
+      |-ideal- <(st, ast, b, DStep :: ds)> =[ if be then c1 else c2 end ]=>
+        <(st', ast', b', os1++[OBranch (beval st be && (negb b))])>
+  | Ideal_If_F : forall st ast b st' ast' b' be c1 c2 os1 ds,
+      |-ideal- <(st, ast, true, ds)> =[ c1 ]=> <(st', ast', b', os1)> ->
+      |-ideal- <(st, ast, b, DForce :: ds)> =[ if be then c1 else c2 end ]=>
+        <(st', ast', b', os1++[OBranch false])>
+  | Ideal_While : forall be st ast b ds st' ast' b' os c,
+      |-ideal- <(st, ast, b, ds)> =[ if be then c; while be do c end else skip end ]=>
+        <(st', ast', b', os)> ->
+      |-ideal- <(st, ast, b, ds)> =[ while be do c end ]=> <(st', ast', b', os)>
+  | Ideal_ARead : forall st ast b x a ie i,
+      aeval st ie = i ->
+      i < length (ast a) ->
+      |-ideal- <(st, ast, b, [DStep])> =[ x <- a[[ie]] ]=>
+        <(x !-> if b then nth 0 (ast a) 0 else nth i (ast a) 0; st, ast, b, [OARead a i])>
+  | Ideal_ARead_U : forall st ast x a ie i a' i',
+      aeval st ie = i ->
+      i >= length (ast a) ->
+      i' < length (ast a') ->
+      |-ideal- <(st, ast, true, [DLoad a' i'])> =[ x <- a[[ie]] ]=>
+        <(x !-> nth 0 (ast a') 0; st, ast, true, [OARead a i])>
+  | Ideal_Write : forall st ast b a ie i e n,
+      aeval st e = n ->
+      aeval st ie = i ->
+      i < length (ast a) ->
+      |-ideal- <(st, ast, b, [DStep])> =[ a[ie] <- e ]=>
+        <(st, a !-> if b then upd 0 (ast a) n else upd i (ast a) n; ast, b, [OAWrite a i])>
+  | Ideal_Write_U : forall st ast a ie i e n a' i',
+      aeval st e = n ->
+      aeval st ie = i ->
+      i >= length (ast a) ->
+      i' < length (ast a') ->
+      |-ideal- <(st, ast, true, [DStore a' i'])> =[ a[ie] <- e ]=>
+        <(st, a' !-> upd 0 (ast a') n; ast, true, [OAWrite a i])>
+
+  where "|-ideal- <( st , ast , b , ds )> =[ c ]=> <( stt , astt , bb , os )>" :=
+    (ideal_eval c st ast b ds stt astt bb os).
+
+Definition ideal_obs_secure c st1 st2 ast1 ast2 : Prop :=
   forall ds stt1 stt2 astt1 astt2 bt1 bt2 os1 os2,
-    <(st1, ast1, false, ds)> =[ c ]=> <(stt1, astt1, bt1, os1)> ->
-    <(st2, ast2, false, ds)> =[ c ]=> <(stt2, astt2, bt2, os2)> ->
+    |-ideal- <(st1, ast1, false, ds)> =[ c ]=> <(stt1, astt1, bt1, os1)> ->
+    |-ideal- <(st2, ast2, false, ds)> =[ c ]=> <(stt2, astt2, bt2, os2)> ->
     os1 = os2.
 
 Lemma relative_noninterference : forall c st1 st2 ast1 ast2,
@@ -112,7 +168,54 @@ Lemma relative_noninterference : forall c st1 st2 ast1 ast2,
   st1 "b" = 1 ->
   st2 "b" = 1 ->
   seq_obs_secure c st1 st2 ast1 ast2 ->
-  ideal_spec_obs_secure c st1 st2 ast1 ast2.
+  ideal_obs_secure c st1 st2 ast1 ast2.
+Proof.
+Admitted.
+
+Definition ultimate_slh_bcc_prop (c: com) (ds :dirs) :Prop :=
+  forall st ast (b: bool) st' ast' b' os,
+    unused "b" c ->
+    st "b" = (if b then 1 else 0) ->
+    <(st, ast, b, ds)> =[ ultimate_slh c ]=> <(st', ast', b', os)> ->
+    |-ideal- <(st, ast, b, ds)> =[ c ]=> <("b" !-> st "b"; st', ast', b', os)>.
+
+Lemma ultimate_slh_bcc : forall c ds,
+  ultimate_slh_bcc_prop c ds.
+Proof.
+  apply prog_size_ind. unfold ultimate_slh_bcc_prop.
+  intros c ds IH st ast b st' ast' b' os Hunused Hstb Heval.
+  destruct c; simpl in *; inversion Heval; subst; clear Heval.
+  - (* Skip *)
+    rewrite t_update_same. apply Ideal_Skip.
+  - (* Asgn *) 
+    rewrite t_update_permute; [| tauto].
+    rewrite t_update_same.
+    constructor. reflexivity.
+  - (* Seq *) 
+    eapply Ideal_Seq.
+    + apply IH in H1; try tauto.
+      * eassumption.
+      * prog_size_auto.
+    + admit. (* needs ultimate_slh_flag lemma
+      apply sel_slh_flag in H1 as Hstb'0; try tauto.
+      apply IH in H10; try tauto.
+      * eapply ideal_unused_update_rev; try tauto.
+      * prog_size_auto. *)
+  (* IF *)
+  - (* non-speculative *) 
+    destruct (beval st <{{ be && "b" = 0 }}>) eqn:Eqnbe; inversion H10; 
+    inversion H1; subst; clear H10; clear H1; simpl in *.
+    + apply andb_true_iff in Eqnbe as [Eqnbe Temp].
+      rewrite Hstb in Temp. destruct b'0 eqn:Hbit; [discriminate |]; clear Temp.
+      apply IH in H11; try tauto.
+      * replace (OBranch true) with (OBranch (beval st be && (negb b'0)))
+          by (rewrite Eqnbe; rewrite Hbit; reflexivity).
+        rewrite <- Hbit at 1. apply Ideal_If. subst. rewrite Eqnbe; simpl.
+          rewrite Eqnbe in H11. rewrite t_update_same in H11.
+          rewrite app_nil_r. apply H11.
+      * prog_size_auto.
+      * rewrite t_update_eq. rewrite Eqnbe. assumption.
+    + (* analog to true case *) admit.
 Admitted.
 
 Theorem relative_secure_slh :
@@ -123,3 +226,5 @@ Theorem relative_secure_slh :
     st2 "b" = 0 ->
     relative_secure ultimate_slh c st1 st2.
 Admitted. (* from relative noninterference + bcc *)
+
+
